src/dvspec/dafny/att_spec_proofs/assump.dfy
@@ -1,0 +1,94 @@
+include "../commons.dfy"
+include "../specification/dvc_spec.dfy"
+include "../specification/consensus.dfy"
+include "../specification/network.dfy"
+include "../specification/dvn.dfy"
+include "../att_spec_proofs/inv.dfy"
+
+module AttAssumptions
+{
+    import opened Types 
+    import opened CommonFunctions
+    import opened ConsensusSpec
+    import opened NetworkSpec
+    import opened DVCNode_Spec
+    import opened DV
+    import opened AttInvariants
+    
+    lemma {:axiom}  monotonic_seq_of_rcvd_att_duties<D(!new, 0)>(
+        dvn: DVState,
+        pubkey: BLSPubkey,
+        s: DVCNodeState,
+        new_att_duty: AttestationDuty)       
+    requires is_honest_node(dvn, pubkey) && s == dvn.honest_nodes_states[pubkey]
+    requires f_serve_attestation_duty.requires(s, new_att_duty)
+    ensures || !s.latest_attestation_duty.isPresent()
+            || ( && s.latest_attestation_duty.isPresent()
+                 && s.latest_attestation_duty.safe_get().slot < new_att_duty.slot 
+               )
+    
+    lemma {:axiom}  rcvd_att_duties_is_prefix_of_global_att_duties<D(!new, 0)>(
+        dvn: DVState,
+        pubkey: BLSPubkey,
+        s: DVCNodeState,
+        new_att_duty: AttestationDuty)       
+    requires is_honest_node(dvn, pubkey) && s == dvn.honest_nodes_states[pubkey]
+    requires f_serve_attestation_duty.requires(s, new_att_duty)
+    ensures || ( exists p1: BLSPubkey :: 
+                    && is_honest_node(dvn, p1)
+                    && var s1 := dvn.honest_nodes_states[p1];
+                    && s1.latest_attestation_duty.isPresent()
+                    && s1.latest_attestation_duty.safe_get() == new_att_duty
+               )
+            || ( forall p1: BLSPubkey :: 
+                    && is_honest_node(dvn, p1)
+                    && var s1 := dvn.honest_nodes_states[p1];                    
+                    && ( || !s1.latest_attestation_duty.isPresent()
+                         || ( && s1.latest_attestation_duty.isPresent()
+                              && s1.latest_attestation_duty.safe_get().slot < new_att_duty.slot
+                            )
+                       )
+               )
+    ensures ! ( exists duty: AttestationDuty ::
+                    && ! ( duty in s.all_rcvd_duties ) 
+                    && duty.slot < new_att_duty.slot
+                    && exists p1: BLSPubkey :: 
+                            ( && is_honest_node(dvn, p1)
+                              && var s1 := dvn.honest_nodes_states[p1];                     
+                              && duty in s1.all_rcvd_duties
+                            )
+              )
+    
+  lemma {:axiom} constructable_signed_attestation_signature(
+    dvn: DVState,
+    att_shares: set<AttestationShare>) 
+  ensures dvn.construct_signed_attestation_signature(att_shares).isPresent()
+            <==> exists S: set<AttestationShare> ::
+                    && S <= att_shares
+                    && |dvn.adversary.nodes| * 2 + 1 <= |S|
+                    && ( forall s1, s2: AttestationShare ::
+                            && s1 in S
+                            && s2 in S
+                                ==> att_shares_from_same_att_data(s1, s2) )
+
+  lemma {:axiom} agreement_on_constructed_signed_attestation_signature(
+    dvn: DVState,
+    att_shares1: set<AttestationShare>, 
+    att_shares2: set<AttestationShare>) 
+  ensures ( && dvn.construct_signed_attestation_signature(att_shares1).isPresent()
+            && dvn.construct_signed_attestation_signature(att_shares2).isPresent()
+            && dvn.construct_signed_attestation_signature(att_shares1).safe_get()
+                  == dvn.construct_signed_attestation_signature(att_shares2).safe_get()
+          )
+            <==> exists S: set<AttestationShare> ::
+                    && S <= att_shares1
+                    && S <= att_shares2
+                    && |dvn.adversary.nodes| * 2 + 1 <= |S|
+                    && ( forall s1, s2: AttestationShare ::
+                            && s1 in S
+                            && s2 in S
+                                ==> att_shares_from_same_att_data(s1, s2) )                                
+}
+
+
+
