src/dvspec/dafny/att_spec_proofs/core_proofs.dfy
@@ -1,0 +1,100 @@
+include "../commons.dfy"
+include "../specification/dvc_spec.dfy"
+include "../specification/consensus.dfy"
+include "../specification/network.dfy"
+include "../specification/dvn.dfy"
+include "../att_spec_proofs/inv.dfy"
+
+module Core_Proofs
+{
+    import opened Types 
+    import opened CommonFunctions
+    import opened ConsensusSpec
+    import opened NetworkSpec
+    import opened DVCNode_Spec
+    import opened DV
+    import opened AttInvariants
+
+/*
+    lemma core_invariants_imply_safety(dvn: DVState)
+    requires pred37c_in_sec_3_8(dvn)    
+    requires pred40(dvn)
+    // ensures safety(dvn)
+    {
+        var pubkey: BLSPubkey :| 
+                && is_honest_node(dvn, pubkey)
+                && dvn.globally_signed_attestations <= seqToSet(dvn.honest_nodes_states[pubkey].bn.attestations_submitted);
+        var s := dvn.honest_nodes_states[pubkey];                
+        var attestations := seqToSet(s.bn.attestations_submitted);
+        var unchecked_attestations := dvn.globally_signed_attestations;
+        var checked_attestations: set<Attestation> := {};
+        
+        while unchecked_attestations != {}
+            invariant unchecked_attestations <= dvn.globally_signed_attestations
+            invariant unchecked_attestations + checked_attestations == dvn.globally_signed_attestations
+            invariant dvn.globally_signed_attestations <= attestations 
+            decreases |unchecked_attestations|
+        {
+            var a: Attestation :| a in unchecked_attestations;
+            assert a in dvn.globally_signed_attestations;
+            assert a in attestations;
+
+            var tempSet := dvn.globally_signed_attestations - { a };
+            assert tempSet <= attestations;
+
+            unchecked_attestations := unchecked_attestations - { a };   
+            checked_attestations := checked_attestations + { a };
+        }
+    }
+    */
+    
+    lemma  lem_1(dvn: DVState)
+    ensures safety(dvn)
+
+    lemma core_invariants_imply_safety(dvn: DVState)
+    requires pred37c_in_sec_3_8(dvn)    
+    requires pred40(dvn)
+    ensures safety(dvn)
+    {
+        var pubkey: BLSPubkey :| 
+                && is_honest_node(dvn, pubkey)
+                && dvn.globally_signed_attestations <= seqToSet(dvn.honest_nodes_states[pubkey].bn.attestations_submitted);
+        var s := dvn.honest_nodes_states[pubkey];                
+        var attestations := seqToSet(s.bn.attestations_submitted);
+        assert dvn.globally_signed_attestations <= attestations;
+
+        var unchecked_attestations := dvn.globally_signed_attestations;
+        var checked_attestations: set<Attestation> := {};
+
+        while unchecked_attestations != {}
+            invariant unchecked_attestations <= dvn.globally_signed_attestations
+            invariant unchecked_attestations + checked_attestations == dvn.globally_signed_attestations
+            invariant dvn.globally_signed_attestations <= attestations 
+            invariant is_honest_node(dvn, pubkey)
+            invariant forall a: Attestation :: 
+                            a in checked_attestations 
+                                ==> && var tempSet := dvn.globally_signed_attestations - { a };
+                                    && is_slashable_attestation_data_in_set_of_attestations(tempSet, a.data);
+            decreases |unchecked_attestations|
+        {
+            var a: Attestation :| a in unchecked_attestations;
+            assert a in dvn.globally_signed_attestations;
+            assert a in attestations;
+
+            var tempSet := dvn.globally_signed_attestations - { a };
+            assert tempSet <= attestations;
+
+            assert is_slashable_attestation_data_in_set_of_attestations(tempSet, a.data);
+
+            unchecked_attestations := unchecked_attestations - { a };   
+            checked_attestations := checked_attestations + { a };
+        }
+        
+
+        assert checked_attestations == dvn.globally_signed_attestations;
+        assert forall a: Attestation :: 
+                    a in dvn.globally_signed_attestations
+                        ==> && var tempSet := dvn.globally_signed_attestations - { a };
+                            && is_slashable_attestation_data_in_set_of_attestations(tempSet, a.data);
+    }
+}
