src/dvspec/dafny/att_spec_proofs/ind_inv.dfy
@@ -1,0 +1,65 @@
+include "../commons.dfy"
+include "../specification/dvc_spec.dfy"
+include "../specification/consensus.dfy"
+include "../specification/network.dfy"
+include "../specification/dvn.dfy"
+include "../att_spec_proofs/inv.dfy"
+
+module AttInductiveInvariants
+{
+    import opened Types 
+    import opened CommonFunctions
+    import opened ConsensusSpec
+    import opened NetworkSpec
+    import opened DVCNode_Spec
+    import opened DV
+    import opened AttInvariants
+
+    predicate att_ind_inv<D(!new, 0)>(dvn: DVState)
+    {
+        && forall i: Slot :: no_conflict_decisions_pred1_in_sec_3_1(dvn.consensus_on_attestation_data[i])
+        && forall i: Slot :: no_decisions_pred2_in_sec_3_1(dvn.consensus_on_attestation_data[i])
+        && consistant_att_slashing_databases_between_honest_nodes_pred3_in_sec_3_2<D>(dvn)
+        && consistant_attestations_in_one_slashing_db_pred4_in_sec_3_2<D>(dvn)
+        && curr_att_duty_is_last_served_duty_pred5_in_sec_3_3<D>(dvn)       
+        && exisiting_consensus_instance_for_curr_att_duty_pred6_in_sec_3_3<D>(dvn)       
+        && active_consensus_instances_imples_existence_of_curr_att_duty_pred7_in_sec_3_3<D>(dvn)       
+        && queued_duties_later_than_curr_att_duty_pred8_in_sec_3_3<D>(dvn)       
+        && submitted_att_by_curr_att_duty_pred9_in_sec_3_3<D>(dvn)       
+        && none_latest_att_duty_implies_empty_att_duty_queue_pred10_in_sec_3_4<D>(dvn)       
+        && queued_duties_later_than_latest_att_duty_pred11_in_sec_3_4<D>(dvn)       
+        && submitted_att_by_latest_att_duty_pred12_in_sec_3_4<D>(dvn)       
+        && active_consensus_instances_for_slots_until_latest_att_duty_pred13_in_sec_3_4<D>(dvn)       
+        && no_active_consensus_instances_for_queued_att_duties_pred14_in_sec_3_5<D>(dvn)       
+        && att_from_imported_block_is_decided_value_pred16_in_sec_3_6<D>(dvn)       
+        && old_duty_has_submitted_att_data_pred17_in_sec_3_6<D>(dvn)       
+        && AttConsensusDecided_is_decided_value_pred18_in_sec_3_7<D>(dvn)       
+        && local_active_consensus_instance_not_later_than_latest_duty_pred19a_in_sec_3_7<D>(dvn)       
+        && no_latest_duty_is_older_than_distributed_undecided_consensus_instance_pred19b_in_sec_3_7<D>(dvn)       
+        && strictly_monotonic_att_duties_queue_pred20_in_sec_3_7<D>(dvn)       
+        && constructable_set_of_att_shares_has_at_least_one_share_from_honest_node_pred21_in_sec_3_7<D>(dvn)       
+        && no_missing_att_in_db_pred22_in_sec_3_7<D>(dvn)       
+        && no_missing_att_in_db_pred23_in_sec_3_7<D>(dvn)       
+        && pred24<D>(dvn)
+        && pred25_in_sec_3_7<D>(dvn)  
+        && sent_att_share_from_honest_node_pred26_in_sec_3_7<D>(dvn)       
+        && undecided_dist_consensus_instance_implies_latest_att_duty_pred27_in_sec_3_7<D>(dvn)       
+        && at_most_one_undecided_dist_consensus_instance_pred28_in_sec_3_7<D>(dvn)       
+        && shared_rcvd_att_duties_pred29_in_sec_3_7<D>(dvn)      
+        && same_function_to_reconstruct_attestations_pred30_in_sec_3_7<D>(dvn) 
+    }
+    
+
+
+
+/*
+    predicate fixed_set_all_nodes_in_sec_3_7<D(!new, 0)>(
+        s: DVCNodeState, 
+        e: Types.Event,
+        s': DVCNodeState)
+    requires f_process_event.requires(s, e)
+    {
+        s' == DVCNode_Spec.f_process_event(s, e).state ==> s.peers == s'.peers                
+    }
+    */
+}
