src/dvspec/dafny/att_spec_proofs/init_implies_ind_inv.dfy
@@ -1,0 +1,68 @@
+include "../commons.dfy"
+include "../specification/dvc_spec.dfy"
+include "../specification/consensus.dfy"
+include "../specification/network.dfy"
+include "../specification/dvn.dfy"
+include "../att_spec_proofs/inv.dfy"
+
+module Init_IndInv
+{
+    import opened Types 
+    import opened CommonFunctions
+    import opened ConsensusSpec
+    import opened NetworkSpec
+    import opened DVCNode_Spec
+    import opened DV
+    import opened AttInvariants
+    
+    lemma init_implies_inv1(dvn: DVState)       
+    requires exists initial_attestation_slashing_db: set<SlashingDBAttestation> :: 
+                DV.Init(dvn, initial_attestation_slashing_db)        
+    ensures forall i: Slot :: no_conflict_decisions_pred1_in_sec_3_1(dvn.consensus_on_attestation_data[i])
+    {}
+
+    lemma honest_node_inconsensus_init_satisfies_inv2<D(!new, 0)>(
+        s: ConsensusInstance, 
+        all_nodes: set<BLSPubkey>, 
+        honest_nodes: set<BLSPubkey>,
+        n: BLSPubkey)
+    requires ConsensusSpec.Init(s, all_nodes, honest_nodes)
+    requires ConsensusSpec.isConditionForSafetyTrue(s)
+    requires n in s.honest_nodes_status.Keys
+    ensures s.honest_nodes_status[n] == NOT_DECIDED
+    { 
+        assert forall t | t in s.honest_nodes_status.Values :: t == NOT_DECIDED;
+        assert s.honest_nodes_status[n] in s.honest_nodes_status.Values;
+        assert s.honest_nodes_status[n] == NOT_DECIDED;
+    }       
+
+
+    lemma consensus_init_implies_inv2<D(!new, 0)>(
+        s: ConsensusInstance, 
+        all_nodes: set<BLSPubkey>, 
+        honest_nodes: set<BLSPubkey>)
+    requires ConsensusSpec.Init(s, all_nodes, honest_nodes)
+    requires ConsensusSpec.isConditionForSafetyTrue(s)    
+    ensures no_decisions_pred2_in_sec_3_1(s)
+    { 
+        var unchecked_honest_nodes := honest_nodes;
+        var checked_honest_nodes := {};
+
+        while unchecked_honest_nodes != {}
+            invariant honest_nodes == unchecked_honest_nodes + checked_honest_nodes
+            invariant unchecked_honest_nodes * checked_honest_nodes == {}
+            invariant checked_honest_nodes <= honest_nodes
+            invariant unchecked_honest_nodes <= honest_nodes
+            invariant forall i: BLSPubkey | i in checked_honest_nodes :: s.honest_nodes_status[i] == NOT_DECIDED
+            decreases |unchecked_honest_nodes|
+        {
+            var i :| i in unchecked_honest_nodes;
+            honest_node_inconsensus_init_satisfies_inv2(s, all_nodes, honest_nodes, i);
+            unchecked_honest_nodes := unchecked_honest_nodes - {i};
+            checked_honest_nodes := checked_honest_nodes + {i};
+        }
+    }       
+}
+
+
+
